WIP multiplexing

src/tls/experiments/TLS.Store.fst
@@ -25,45 +25,135 @@ let store_regions_disjoint i j = ()
 
 let tls_store_server_cookie_region = List.Tot.index store_regions 0
 let tls_store_server_ticket_region = List.Tot.index store_regions 1
+let tls_store_wrap_psk_region = List.Tot.index store_regions 2
+let tls_store_client_seal_region = List.Tot.index store_regions 3
 
 let loc_store_regions_disjoint = ()
 
+let tls_store_regions (u: usage) : Tot substore =
+  match u with
+  | ServerCookie -> tls_store_server_cookie_region
+  | ServerTicket -> tls_store_server_ticket_region
+  | ClientSeal -> tls_store_client_seal_region
+  | WrapPSK -> tls_store_wrap_psk_region
+
+let loc_store_regions (u: usage) : GTot B.loc = B.loc_all_regions_from true (tls_store_regions u)
+
+let loc_store_regions_disjoint' (u1 u2: usage) : Lemma
+  (requires (u1 <> u2))
+  (ensures (B.loc_disjoint (loc_store_regions u1) (loc_store_regions u2)))
+  [SMTPat (B.loc_disjoint (loc_store_regions u1) (loc_store_regions u2))]
+= ()
+
 assume val server_cookie_phi : AE.plain_pred 
-
-let server_cookie_key :
-  (server_cookie_key: B.pointer (option (a: alg & (st: AE.state a server_cookie_phi { B.loc_includes (loc_store_server_cookie_region ()) (AE.footprint st) }))) {
-    B.recallable server_cookie_key /\
-    B.frameOf server_cookie_key == tls_store_server_cookie_region
-  }) = B.gcmalloc tls_store_server_cookie_region None 1ul
-
 assume val server_ticket_phi : AE.plain_pred 
 
-let server_ticket_key :
-  (server_ticket_key: B.pointer (option (a: alg & (st: AE.state a server_ticket_phi { B.loc_includes (loc_store_server_ticket_region ()) (AE.footprint st) }))) {
-    B.recallable server_ticket_key /\
-    B.frameOf server_ticket_key == tls_store_server_ticket_region
-  }) = B.gcmalloc tls_store_server_ticket_region None 1ul
+let phi (u: usage) : Tot AE.plain_pred =
+  match u with
+  | ServerCookie -> server_cookie_phi
+  | ServerTicket -> server_ticket_phi
+  | _ -> server_cookie_phi
 
-unfold
-let inv' (h: HS.mem) : Tot Type0 =
-  B.live h server_cookie_key /\
-  begin match B.deref h server_cookie_key with
+inline_for_extraction
+noextract
+let ptr (u: usage) : Tot Type0 =
+  (ptr: B.pointer (option (a: alg & (st: AE.state a (phi u) { B.loc_includes (loc_store_regions u) (AE.footprint st) }))) {
+    B.recallable ptr /\
+    B.frameOf ptr == tls_store_regions u
+  })
+
+let server_cookie_key : ptr ServerCookie =
+  B.gcmalloc tls_store_server_cookie_region None 1ul
+
+let server_ticket_key : ptr ServerTicket =
+  B.gcmalloc tls_store_server_ticket_region None 1ul
+
+let wrap_psk_key : ptr WrapPSK =
+  B.gcmalloc tls_store_wrap_psk_region None 1ul
+
+let client_seal_key : ptr ClientSeal =
+  B.gcmalloc tls_store_client_seal_region None 1ul
+
+inline_for_extraction
+let keyptr (u: usage) : Tot (ptr u) =
+  match u with
+  | ServerCookie -> server_cookie_key
+  | ServerTicket -> server_ticket_key
+  | WrapPSK -> wrap_psk_key
+  | ClientSeal -> client_seal_key
+
+let per_usage_inv (h: HS.mem) (u: usage) : Tot Type0 =
+  B.live h (keyptr u) /\
+  begin match B.deref h (keyptr u) with
   | None -> True
   | Some (| a, st |) ->
-    B.loc_disjoint (AE.footprint st) (B.loc_buffer server_cookie_key) /\
-    AE.invariant h st
-  end /\
-  B.live h server_ticket_key /\
-  begin match B.deref h server_ticket_key with
-  | None -> True
-  | Some (| a, st |) ->
-    B.loc_disjoint (AE.footprint st) (B.loc_buffer server_ticket_key) /\
+    B.loc_disjoint (AE.footprint st) (B.loc_buffer (keyptr u)) /\
     AE.invariant h st
   end
 
+unfold
+let inv' (h: HS.mem) : Tot Type0 =
+  per_usage_inv h ServerCookie /\
+  per_usage_inv h ServerTicket /\
+  per_usage_inv h WrapPSK /\
+  per_usage_inv h ClientSeal
+
 let inv = inv'
 
+let per_usage_frame'
+  (u u': usage)
+  (h: HS.mem)
+  (l: B.loc)
+  (h' : HS.mem)
+: Lemma
+  (requires (
+    u <> u' /\
+    per_usage_inv h u' /\
+    B.modifies (loc_store_regions u `B.loc_union` l) h h' /\
+    B.loc_disjoint l (Mem.loc_store_region ())
+  ))
+  (ensures (per_usage_inv h' u'))
+= admit ()
+
+let per_usage_frame
+  (u: usage)
+  (h: HS.mem)
+  (l: B.loc)
+  (h' : HS.mem)
+: Lemma
+  (requires (
+    inv h /\
+    B.modifies (loc_store_regions u `B.loc_union` l) h h' /\
+    B.loc_disjoint l (Mem.loc_store_region ()) /\
+    per_usage_inv h' u
+  ))
+  (ensures (inv h'))
+= match u with
+  | ServerCookie ->
+    per_usage_frame' ServerCookie WrapPSK h l h';
+    per_usage_frame' ServerCookie ServerTicket h l h';
+    per_usage_frame' ServerCookie ClientSeal h l h'
+  | ServerTicket ->
+    per_usage_frame' ServerTicket WrapPSK h l h';
+    per_usage_frame' ServerTicket ServerCookie h l h';
+    per_usage_frame' ServerTicket ClientSeal h l h'
+  | WrapPSK ->
+    per_usage_frame' WrapPSK ServerTicket h l h';
+    per_usage_frame' WrapPSK ServerCookie h l h';
+    per_usage_frame' WrapPSK ClientSeal h l h'
+  | ClientSeal ->
+    per_usage_frame' ClientSeal ServerTicket h l h';
+    per_usage_frame' ClientSeal ServerCookie h l h';
+    per_usage_frame' ClientSeal WrapPSK h l h'
+
 let frame h l h' =
+  per_usage_frame' ServerCookie WrapPSK h l h' ;
+  per_usage_frame' WrapPSK ServerTicket h l h' ;
+  per_usage_frame' ServerTicket ClientSeal h l h' ;
+  per_usage_frame' ClientSeal ServerCookie h l h'
+
+(*
+
   assert (Mem.loc_store_region () `B.loc_includes` B.loc_buffer server_cookie_key);
   assert (Mem.loc_store_region () `B.loc_includes` B.loc_buffer server_ticket_key); 
   assert (B.live h' server_cookie_key);
